Checkpoint etcd client progress

new/proof/context.v
@@ -3,25 +3,52 @@ Require Import New.generatedproof.context.
 Require Import New.proof.proof_prelude.
 
 Require Import Perennial.Helpers.CountableTactics.
-Section definitions.
+
+Section chan.
 
 Context `{hG: heapGS Σ, !ffi_semantics _ _}.
+Axiom own_chan :
+  ∀ `{!IntoVal V} (c : chan.t) (buf : list V) (unbuf_entry : option V) (closed : bool), iProp Σ.
 
+End chan.
+
+Module Context_state.
+Section defn.
+Context `{ffi_syntax}.
 (* FIXME: prove this and put it in golang directory. *)
 Instance interface_countable : Countable interface.t.
 Admitted.
 
-(* spec-level state of a Context is:
-   Values : gmap
- *)
-Record state :=
-  {
-    Values : gmap interface.t interface.t;
-    (* FIXME: *)
-    (* Deadline : time.Time.t  *)
-    Deadline : option w64;
-    Done: chan.t;
-  }.
+Record t :=
+  mk
+    {
+      Values : gmap interface.t interface.t;
+      (* FIXME: *)
+      (* Deadline : time.Time.t  *)
+      Deadline : option w64;
+      Done: chan.t;
+    }.
+End defn.
+End Context_state.
+
+Section definitions.
+
+Context `{hG: heapGS Σ, !ffi_semantics _ _}.
+
+Import Context_state.
+Definition is_Context (c : interface.t) (s : Context_state.t) : iProp Σ :=
+  "#HDeadline" ∷
+    {{{ True }}}
+      interface.get #"Deadline" #c #()
+    {{{ RET (#(default (W64 0) s.(Deadline)),
+             #(match s.(Deadline) with | None => false | _ => true end));
+        True
+    }}} ∗
+  "#HDone" ∷
+    {{{ True }}}
+      interface.get #"Done" #c #()
+    {{{ RET #s.(Done); True }}}.
+
 (*
 From the docs for `WithCancel`:
  The returned context's Done channel is closed when the returned cancel function
@@ -36,17 +63,17 @@ So, cannot prove that calling `cancel` actually causes anything to happen; that
 would be a liveness property. But should be able to do the converse.
 
 Should be able to prove that if the returned context's Done channel is closed,
-then (cancel was run) ∨ (chan.is_closed ctx.Done).
+then (cancel was run) ∨ (chan.is_closed ctx.Done). *)
 
-Perhaps there should be a "done" predicate associated with channels? A thing
-that must be true before a chan can be closed.
-
-{{{ True }}}
-  WithCancel(ctx)
-{{{
-  RET (#ctx, #cancel);
-}}}
-
-*)
+Lemma wp_WithCancel N (ctx : interface.t) :
+  {{{ True }}}
+    func_call #context.pkg_name' #"WithCancel" #ctx
+  {{{
+        ctx' ctx_state (cancel : func.t), RET (#ctx', #cancel);
+        is_Context ctx' ctx_state ∗
+        inv N (∃ closed, own_chan ctx_state.(Done) ([] : list unit) None closed)
+  }}}.
+Proof.
+Admitted.
 
 End definitions.
