new/proof/go_etcd_io/etcd/client/v3.v
@@ -1,0 +1,54 @@
+Require Import New.code.go_etcd_io.etcd.client.v3.
+Require Import New.generatedproof.go_etcd_io.etcd.client.v3.
+Require Import New.proof.proof_prelude.
+
+(** Notes about the etcd robustness test model.
+ - The real `Lease.Grant()` does not take in a LeaseID, it gets it from the server.
+   The model, on the other hand, uses the LeaseID straight from the LeaseGrant
+   request (even if the LeaseID were zero, which indicates to the LeaseGrant RPC
+   that the lessor should choose an ID).
+*)
+
+Module EtcdState.
+Record t :=
+mk {
+    Revision : w64;
+    CompactRevision : w64;
+    KeyValues : gmap string (string * w64);
+    KeyLeases : gmap string w64;
+    Leases : gmap w64 (w64 * gset string);
+  }.
+
+Global Instance settable_EtcdState : Settable _ :=
+  settable! EtcdState.mk < Revision; CompactRevision; KeyValues; KeyLeases; Leases >.
+End EtcdState.
+
+
+Definition is_Grant (leaseid) (s s' : EtcdState.t) : Prop :=
+  let leaase := LeaseId
+.
+
+
+Module RangeRequest.
+Record t :=
+mk {
+    Revision : w64;
+    Start : go_string;
+    End : go_string;
+    Limit : w64;
+  }.
+End RangeRequest.
+
+Definition get_range (start end : go_string) (limit : w64) (s : EtcdState.t) : Prop :=
+.
+
+Definition range_operation (request : RangeRequest.t) (s s' : EtcdState.t) : Prop :=
+  if decide (request.(RangeRequest.Revision) = 0 ∨
+             request.(RangeRequest.Revision) = s.(EtcdState.Revision))
+  then
+    True
+  else if decide (request.(RangeRequest.Revision) > s.(EtcdState.Revision)) then
+         True
+       else
+         True
+.
