new/proof/go_etcd_io/etcd/client/v3/concurrency.v
@@ -1,6 +1,7 @@
 Require Import New.code.go_etcd_io.etcd.client.v3.concurrency.
 Require Import New.generatedproof.go_etcd_io.etcd.client.v3.concurrency.
 Require Import New.proof.proof_prelude.
+Require Import New.proof.context.
 
 Section proof.
 
@@ -80,27 +81,19 @@ Proof.
   wp_alloc client_ptr as "Hclient_ptr".
   wp_pures.
   wp_alloc lg_ptr as "Hlg_ptr".
-  wp_pures.
-  wp_load.
+  wp_pures. wp_load.
   wp_apply (wp_Client__GetLogger with "[$]").
   iIntros (?) "_".
-  wp_pures.
-  wp_store.
-  wp_pures.
+  wp_pures. wp_store. wp_pures.
   wp_alloc ops_ptr as "Hops_ptr".
-  wp_pures.
-  wp_load.
+  wp_pures. wp_load.
   wp_apply (wp_Client__Ctx with "[$]").
   iIntros (?) "_".
   wp_pures.
   wp_alloc ops as "Hops".
-  wp_pures.
-  wp_store.
-  wp_pures.
+  wp_pures. wp_store. wp_pures.
   wp_alloc opt_ptr as "Hopt_ptr".
-  wp_pures.
-  wp_load.
-  wp_pures.
+  wp_pures. wp_load. wp_pures.
 
   (* only consider nil options *)
   wp_apply wp_slice_for_range.
@@ -112,39 +105,17 @@ Proof.
 
   wp_pures.
   wp_alloc id_ptr as "Hid_ptr".
-  wp_pures.
-  wp_load.
-  wp_pures.
-  wp_load.
-  wp_pures.
-  wp_store.
-  wp_pures.
-  wp_load.
+  wp_pures. wp_load. wp_pures. wp_load. wp_pures. wp_store. wp_pures. wp_load.
 
   (* id == clientv3.NoLease, so call `Grant` *)
   wp_pures.
   wp_alloc err_ptr as "Herr_ptr".
   wp_pures.
   wp_alloc resp_ptr as "Hresp_ptr".
-  wp_pures.
-  wp_load.
-  wp_pures.
-  wp_load.
-  wp_pures.
-  wp_load.
-  wp_pures.
-  wp_load.
-  wp_pures.
-  wp_load.
+  wp_pures. wp_load. wp_pures. wp_load. wp_pures. wp_load. wp_pures. wp_load. wp_pures. wp_load.
   wp_apply (wp_Client__Grant with "[$]").
   iIntros "* Hresp".
-  wp_pures.
-  wp_store.
-  wp_pures.
-  wp_store.
-  wp_pures.
-  wp_load.
-  wp_pures.
+  wp_pures. wp_store. wp_pures. wp_store. wp_pures. wp_load. wp_pures.
   destruct bool_decide eqn:Herr.
   2:{ (* got an error; early return *)
     wp_pures.
@@ -155,22 +126,20 @@ Proof.
     rewrite decide_False //.
   }
   (* no error from Grant() call *)
-  wp_pures.
-  wp_load.
-  wp_pures.
-  wp_load.
-  wp_pures.
-  wp_store.
-  wp_pures.
+  wp_pures. wp_load. wp_pures. wp_load. wp_pures. wp_store. wp_pures.
   wp_alloc cancel_ptr as "Hcancel_ptr".
   wp_pures.
   wp_alloc ctx_ptr as "Hctx_ptr".
-  wp_pures.
-  wp_load.
-  wp_pures.
-  wp_load.
-  wp_pures.
-  (* TODO: spec for context.WithCancel *)
+  wp_pures. wp_load. wp_pures. wp_load. wp_pures.
+
+  (* XXX: eventually, this spec will require context.is_initialized *)
+  wp_apply (wp_WithCancel nroot with "[]").
+  iIntros "* [#Hctx #Hctx_done_inv]".
+  wp_pures. wp_store. wp_pures. wp_store. wp_pures.
+  iClear "Herr_ptr". clear err_ptr.
+  wp_alloc err_ptr as "Herr_ptr". wp_pures.
+  wp_alloc keepAlive_ptr as "HkeepAlive_ptr". wp_pures.
+  wp_load. wp_pures. wp_load. wp_pures. wp_load.
 Admitted.
 
 End proof.
